Extended PHOAS to open terms

TypeSoundness.v
@@ -19,13 +19,15 @@ Inductive steps : expr -> expr -> Prop :=
 | StepsS e1 e2 e3 : step e1 e2 -> steps e2 e3 -> steps e1 e3
 .
 
-Definition typingsim T e τ := exists c s, typing T e τ c s.
+Notation "⊢" := typing.
+Definition typingsim T e τ := exists c s, ⊢ T e τ c s.
+Notation "|-" := typingsim.
 
 Definition nostuck e := forall e', steps e e' -> IsValue e' \/ exists e'', step e' e''.
 
 Theorem sound_wrt_nostuck :
   forall e τ,
-    typingsim [] e τ ->
+    |- [] e τ ->
     nostuck e.
 Proof.
   admit.
@@ -100,74 +102,193 @@ Definition asNat P c :=
   (exists nc, nat_of_cexpr c = Some nc /\ P nc)%type.
 Notation "⌊ n | P ⌋" := (asNat (fun n => P)).
 
-(* An Logical Step-indexed Logical Relation (LSLR) for boundedness *)
+Infix "×" := Tprod (at level 40).
+Infix "+" := Tsum.
+Notation "e ↓ τ" := (IsValue e /\ |- [] e τ) (at level 51).
 
-(* A Parametric Higher-Order Abstract Syntax encoding *)
+(* A Parametric Higher-Order Abstract Syntax (PHOAS) encoding for a second-order modal logic (LSLR) *)
 
-Section propR.
+Section rel.
 
   Variable var : nat -> Type.
   
-  Inductive propR : nat -> Type :=
-  | PRvar t : var t -> propR t
-  | PRlift : Prop -> propR 0
-  | PRtrue : propR 0
-  | PRfalse : propR 0
-  | PRand (_ _ : propR 0) : propR 0
-  | PRor (_ _ : propR 0) : propR 0
-  | PRimply (_ _ : propR 0) : propR 0
-  | PRforalle : (expr -> propR 0) -> propR 0
-  | PRexistse : (expr -> propR 0) -> propR 0
-  | PRforallR n : (var n -> propR 0) -> propR 0
-  | PRexistsR n : (var n -> propR 0) -> propR 0
-  | PRforall1 T : (T -> propR 0) -> propR 0
-  | PRexists1 T : (T -> propR 0) -> propR 0
-  | PRabs n : (expr -> propR n) -> propR (S n)
-  | PRapp n : propR (S n) -> expr -> propR n
-  | PRrecur n : (var n -> propR n) -> propR n
-  | PRlater : propR 0 -> propR 0
+  Inductive rel : nat -> Type :=
+  | Rvar n : var n -> rel n
+  | Rlift : Prop -> rel 0
+  | Rtrue : rel 0
+  | Rfalse : rel 0
+  | Rand (_ _ : rel 0) : rel 0
+  | Ror (_ _ : rel 0) : rel 0
+  | Rimply (_ _ : rel 0) : rel 0
+  | Rforalle : (expr -> rel 0) -> rel 0
+  | Rexistse : (expr -> rel 0) -> rel 0
+  | RforallR n : (var n -> rel 0) -> rel 0
+  | RexistsR n : (var n -> rel 0) -> rel 0
+  | Rforall1 T : (T -> rel 0) -> rel 0
+  | Rexists1 T : (T -> rel 0) -> rel 0
+  | Rabs n : (expr -> rel n) -> rel (S n)
+  | Rapp n : rel (S n) -> expr -> rel n
+  | Rrecur n : (var n -> rel n) -> rel n
+  | Rlater : rel 0 -> rel 0
   .
 
-End propR.
+End rel.
 
-Definition PropR n := forall var, propR var n.
+Section relOpen.
 
-Infix "×" := Tprod (at level 40).
-Infix "+" := Tsum.
-Notation "⊢" := typingsim.
+  Variable var : nat -> Type.
+  
+  Fixpoint relOpen R n :=
+    match R with
+      | nil => rel var n 
+      | nv :: R' => var nv -> relOpen R' n
+    end.
 
-Notation "⊤" := (PRtrue _).
-Notation "⊥" := (PRtrue _).
-(* Notation "\ e , p" := (PRabs (fun e => p)) (at level 200, format "\ e , p"). *)
-Notation "\ x .. y , p" := (PRabs (fun x => .. (PRabs (fun y => p)) ..)) (at level 200, x binder, y binder, right associativity).
-Notation "∀ x .. y , p" := (PRforalle (fun x => .. (PRforalle (fun y => p)) ..)) (at level 200, x binder, y binder, right associativity).
-Notation "∃ x .. y , p" := (PRexistse (fun x => .. (PRexistse (fun y => p)) ..)) (at level 200, x binder, y binder, right associativity).
-Notation "∀1 x .. y , p" := (PRforall1 (fun x => .. (PRforall1 (fun y => p)) ..)) (at level 200, x binder, y binder, right associativity).
-Notation "∃1 x .. y , p" := (PRexists1 (fun x => .. (PRexists1 (fun y => p)) ..)) (at level 200, x binder, y binder, right associativity).
-Definition PRforallR' var n P := (@PRforallR var n (fun x => P (PRvar _ _ x))).
-Notation "∀2 x .. y , p" := (PRforallR' (fun x => .. (PRforallR' (fun y => p)) ..)) (at level 200, x binder, y binder, right associativity).
-Definition PRexistsR' var n P := (@PRexistsR var n (fun x => P (PRvar _ _ x))).
-Notation "∃2 x .. y , p" := (PRexistsR' (fun x => .. (PRexistsR' (fun y => p)) ..)) (at level 200, x binder, y binder, right associativity).
-Definition PRrecur' var n P := (@PRrecur var n (fun x => P (PRvar _ _ x))).
-Notation "@ x .. y , p" := (PRrecur' (fun x => .. (PRrecur' (fun y => p)) ..)) (at level 200, x binder, y binder, right associativity).
-Notation "⌈ P ⌉" := (PRlift _ P).
-Notation "e ↓ τ" := (IsValue e /\ ⊢ [] e τ) (at level 51).
-Notation "e ∈ P" := (PRapp P e) (at level 70).
-Infix "/\" := PRand.
-Infix "\/" := PRor.
-Infix "⇒" := PRimply (at level 90).
-Notation "▹" := PRlater.
-Definition VSet var τ (S : propR var 1) := ∀ v, v ∈ S ⇒ ⌈v ↓ τ⌉.
+  Program Fixpoint liftToOpen R n1 n2 (f : rel var n1 -> rel var n2) (a : relOpen R n1) : relOpen R n2 :=
+    match R with
+      | nil => _
+      | nv :: R' => _ (@liftToOpen R' n1 n2)
+    end.
+  Next Obligation.
+    exact (f a).
+  Defined.
+  Next Obligation.
+    exact (x f (a X)).
+  Defined.
 
+  Require Import Program.
+
+  Program Fixpoint liftToOpen2 R n1 n2 T (f : (T -> rel var n1) -> rel var n2) (a : T -> relOpen R n1) : relOpen R n2 :=
+    match R with
+      | nil => _
+      | nv :: R' => _ (@liftToOpen2 R' n1 n2)
+    end.
+  Next Obligation.
+    exact (f a).
+  Defined.
+  Next Obligation.
+    exact (x _ f (flip a X)).
+  Defined.
+
+  Program Fixpoint liftToOpen3 R n T (f : T -> rel var n) (a : T) : relOpen R n :=
+    match R with
+      | nil => _
+      | nv :: R' => _ (@liftToOpen3 R' n)
+    end.
+
+  Program Fixpoint liftToOpen4 R n (f : rel var n) : relOpen R n :=
+    match R with
+      | nil => _
+      | nv :: R' => _ (@liftToOpen4 R' n)
+    end.
+
+  Program Fixpoint liftToOpen5 R n1 n2 n3 (f : rel var n1 -> rel var n2 -> rel var n3) (a : relOpen R n1) (b : relOpen R n2) : relOpen R n3 :=
+    match R with
+      | nil => _
+      | nv :: R' => _ (@liftToOpen5 R' n1 n2 n3)
+    end.
+  Next Obligation.
+    exact (f a b).
+  Defined.
+  Next Obligation.
+    exact (x f (a X) (b X)).
+  Defined.
+
+  Program Fixpoint liftToOpen6 R n1 T n2 (f : rel var n1 -> T -> rel var n2) (a : relOpen R n1) (b : T) : relOpen R n2 :=
+    match R with
+      | nil => _
+      | nv :: R' => _ (@liftToOpen6 R' n1 T n2)
+    end.
+  Next Obligation.
+    exact (f a b).
+  Defined.
+  Next Obligation.
+    exact (x f (a X) b).
+  Defined.
+
+  Variable R : list nat.
+
+  Definition ORvar n := liftToOpen3 R (@Rvar var n).
+  Definition ORlift := liftToOpen3 R (@Rlift var).
+  Definition ORtrue := liftToOpen4 R (@Rtrue var).
+  Definition ORfalse := liftToOpen4 R (@Rfalse var).
+  Definition ORand := liftToOpen5 R (@Rand var).
+  Definition ORor := liftToOpen5 R (@Ror var).
+  Definition ORimply := liftToOpen5 R (@Rimply var).
+  Definition ORforalle := liftToOpen2 R (@Rforalle var).
+  Definition ORexistse := liftToOpen2 R (@Rexistse var).
+  Definition ORforallR n := liftToOpen2 R (@RforallR var n).
+  Definition ORexistsR n := liftToOpen2 R (@RexistsR var n).
+  Definition ORforall1 T := liftToOpen2 R (@Rforall1 var T).
+  Definition ORexists1 T := liftToOpen2 R (@Rexists1 var T).
+  Definition ORabs n := liftToOpen2 R (@Rabs var n).
+  Definition ORapp n := liftToOpen6 R (@Rapp var n).
+  Definition ORrecur n := liftToOpen2 R (@Rrecur var n).
+  Definition ORlater := liftToOpen R (@Rlater var).
+
+End relOpen.
+    
+Notation "⊤" := (ORtrue _ _).
+Notation "⊥" := (ORtrue _ _).
+Notation "⌈ P ⌉" := (ORlift _ _ P).
+Arguments ORabs {var R n} _ .
+Notation "\ x .. y , p" := (ORabs (fun x => .. (ORabs (fun y => p)) ..)) (at level 200, x binder, y binder, right associativity).
+Arguments ORforalle {var R} _ .
+Notation "∀ x .. y , p" := (ORforalle (fun x => .. (ORforalle (fun y => p)) ..)) (at level 200, x binder, y binder, right associativity).
+Arguments ORexistse {var R} _ .
+Notation "∃ x .. y , p" := (ORexistse (fun x => .. (ORexistse (fun y => p)) ..)) (at level 200, x binder, y binder, right associativity).
 Section TestNotations.
   
   Variable var : nat -> Type.
+  Variable R : list nat.
 
-  Definition ttt1 : propR var 1 := \e , ⊤.
-  Definition ttt2 : propR var 1 := \e , ⌈e ↓ Tunit⌉.
-  Definition ttt3 : propR var 1 := \_ , ⌈True /\ True⌉.
+  Definition ttt1 : relOpen var R 1 := \e , ⊤.
+  Definition ttt2 : relOpen var R 1 := \e , ⌈e ↓ Tunit⌉.
+  Definition ttt3 : relOpen var R 1 := \_ , ⌈True /\ True⌉.
+  Definition ttt4 : relOpen var R 1 := \_ , ∀ e, ⌈e = Ett⌉.
+  Definition ttt5 : relOpen var R 1 := \_ , ∃ e, ⌈e = Ett⌉.
 
 End TestNotations.
+
+Arguments ORforall1 {var R T} _ .
+Notation "∀1 x .. y , p" := (ORforall1 (fun x => .. (ORforall1 (fun y => p)) ..)) (at level 200, x binder, y binder, right associativity).
+Arguments ORexists1 {var R T} _ .
+Notation "∃1 x .. y , p" := (ORexists1 (fun x => .. (ORexists1 (fun y => p)) ..)) (at level 200, x binder, y binder, right associativity).
+Definition ORforallR' {var R n} P := (@ORforallR var R n (fun x => P (ORvar var R _ x))).
+Notation "∀2 x .. y , p" := (ORforallR' (fun x => .. (ORforallR' (fun y => p)) ..)) (at level 200, x binder, y binder, right associativity).
+Definition ORexistsR' {var R n} P := (@ORexistsR var R n (fun x => P (ORvar var R _ x))).
+Notation "∃2 x .. y , p" := (ORexistsR' (fun x => .. (ORexistsR' (fun y => p)) ..)) (at level 200, x binder, y binder, right associativity).
+Definition ORrecur' {var R n} P := (@ORrecur var R n (fun x => P (ORvar var R _ x))).
+Notation "@ x .. y , p" := (ORrecur' (fun x => .. (ORrecur' (fun y => p)) ..)) (at level 200, x binder, y binder, right associativity).
+Arguments ORapp {var R n} _ _ .
+Notation "e ∈ P" := (ORapp P e) (at level 70).
+Arguments ORand {var R} _ _ .
+Infix "/\" := ORand.
+Arguments ORor {var R} _ _ .
+Infix "\/" := ORor.
+Arguments ORimply {var R} _ _ .
+Infix "⇒" := ORimply (at level 90).
+Arguments ORlater {var R} _ .
+Notation "▹" := ORlater.
+Definition VSet {var R} τ (S : relOpen var R 1) := ∀ v, v ∈ S ⇒ ⌈v ↓ τ⌉.
+
+(*
+Section inferRules.
+
+  Variable var : nat -> Type.
+
+  Variable R : list nat.
+
+  Definition prop := openRel R 0.
+
+  Fixpoint 
+
+  Inductive valid : list prop -> prop -> Prop :=
+  | Vmono C P : 
+*)
+
+
+(* An Logical Step-indexed Logical Relation (LSLR) for boundedness *)
 
 Inductive thresholds :=
 | THleaf
@@ -183,6 +304,7 @@ Local Open Scope prog_scope.
 Section LR.
   
   Variable var : nat -> Type.
+  Variable R : list nat.
 
   Definition substs : Type.
     admit.
@@ -194,11 +316,11 @@ Section LR.
 
   Coercion substs_type : substs >-> Funclass.
 
-  Definition substs_sem : substs -> nat -> propR var 1.
+  Definition substs_sem : substs -> nat -> relOpen var R 1.
     admit.
   Defined.
 
-  Instance Apply_substs_nat_propR : Apply substs nat (propR var 1) :=
+  Instance Apply_substs_nat_rel : Apply substs nat (relOpen var R 1) :=
     {
       apply := substs_sem
     }.
@@ -230,19 +352,19 @@ Section LR.
       add := add_csize
     }.
 
-  Definition add_pair : (type * propR var 1) -> substs -> substs.
+  Definition add_pair : (type * relOpen var R 1) -> substs -> substs.
     admit.
   Defined.
 
-  Instance Add_pair_substs : Add (type * propR var 1) substs substs :=
+  Instance Add_pair_substs : Add (type * relOpen var R 1) substs substs :=
     {
       add := add_pair
     }.
 
-  Definition E' V τ (c : cexpr) (s : size) (ρ : substs) C (θ : thresholds) : propR var 1 :=
-    \e, ∀ v, ∀1 n, ⌈⊢ [] e (ρ τ) /\ ⇓ e n v⌉ ⇒ ⌈ ⌊ ñ | n ≤ C * ñ ⌋ (ρ $ c) ⌉ /\ ∃1 ξ : csize, ⌈ξ ≤ ρ $$ s⌉ /\ v ∈ V τ ξ ρ C θ.
+  Definition E' V τ (c : cexpr) (s : size) (ρ : substs) C (θ : thresholds) : relOpen var R 1 :=
+    \e, ∀ v, ∀1 n, ⌈|- [] e (ρ τ) /\ ⇓ e n v⌉ ⇒ ⌈ ⌊ ñ | n ≤ C * ñ ⌋ (ρ $ c) ⌉ /\ ∃1 ξ : csize, ⌈ξ ≤ ρ $$ s⌉ /\ v ∈ V τ ξ ρ C θ.
 
-  Fixpoint V τ (ξ : csize) (ρ : substs) (C : nat) (θ : thresholds) {struct τ} : propR var 1 :=
+  Fixpoint V τ (ξ : csize) (ρ : substs) (C : nat) (θ : thresholds) {struct τ} : relOpen var R 1 :=
     match τ, ξ, θ with
       | Tvar α, _, _ => ρ $ α
       | Tunit, _, _ => \v, ⌈v ↓ τ⌉
@@ -260,12 +382,14 @@ Section LR.
 
 End LR.
 
-Definition relV τ ξ ρ C θ : PropR 1 := fun var => V var τ ξ ρ C θ.
-Definition relE τ c s ρ C θ : PropR 1 := fun var => E var τ c s ρ C θ.
+Definition Rel n := forall var R, relOpen var R n.
 
-Theorem sound_wrt_bounded :
+Definition relV τ ξ ρ C θ : Rel 1 := fun var R => V var R τ ξ ρ C θ.
+Definition relE τ c s ρ C θ : Rel 1 := fun var R => E var R τ c s ρ C θ.
+
+Definition sound_wrt_bounded :=
   forall f τ₁ c s τ₂, 
-    ⊢ [] f (Tarrow τ₁ c s τ₂) -> 
+    |- [] f (Tarrow τ₁ c s τ₂) -> 
     exists (C : nat) (ξ₀ : csize), 
       (* ξ₀ is the threshold of input size in asymptotics *)
       forall v,
@@ -277,6 +401,24 @@ Theorem sound_wrt_bounded :
           ⇓ (Eapp f v) n v' ->
           (* n is bounded by c(ξ) w.r.t. constant factor C *)
           ⌊ ñ | n <= C * ñ ⌋ (subst ξ c).
+
+Definition related Γ e τ c s :=
+  (* ⊢ Γ e τ c s /\ *)
+  exists X,
+    wfVarCtx Γ X ->
+    exists R,
+      wfRelCtx Γ R ->
+      
+Lemma foundamental :
+  forall Γ e τ c s,
+    ⊢ Γ e τ c s -> 
+    ⊩ Γ e τ c s.
 Proof.
   admit.
 Qed.
+
+Theorem sound_wrt_bound_proof : sound_wrt_bounded.
+Proof.
+  admit.
+Qed.
+
